Obtain fixpoint substitution with recursor

operations/BMV_Fixpoint.thy
@@ -33,7 +33,7 @@ local_setup \<open>fn lthy =>
     (* Step 4: Construct the binder fixpoint *)
     val (fp_res, lthy) = MRBNF_FP.construct_binder_fp BNF_Util.Least_FP
     [{
-      FVars = replicate 2 NONE,
+      FVars = [SOME "FTVars", SOME "FVars"],
       T_name = "FTerm",
       nrecs = 2,
       permute = NONE,
@@ -46,7 +46,7 @@ local_setup \<open>fn lthy =>
       I @{typ "('tv, 'v, 'btv, 'bv, 'c, 'd) FTerm_pre'"} ([], lthy))
 
     (* Register bmv to access theorems later *)
-    val lthy = BMV_Monad_Def.register_pbmv_monad "FTerm_pre'" bmv lthy;
+    val lthy = BMV_Monad_Def.register_pbmv_monad "BMV_Fixpoint.FTerm_pre'" bmv lthy;
 
     val notes = [
       ("bmv_defs", thms)
@@ -60,7 +60,7 @@ local_setup \<open>fn lthy =>
   in lthy end\<close>
 
 ML \<open>
-val bmv = the (BMV_Monad_Def.pbmv_monad_of @{context} "FTerm_pre'")
+val bmv = the (BMV_Monad_Def.pbmv_monad_of @{context} "BMV_Fixpoint.FTerm_pre'")
 val axioms = BMV_Monad_Def.axioms_of_bmv_monad bmv;
 val laxioms = nth axioms (BMV_Monad_Def.leader_of_bmv_monad bmv)
 \<close>
@@ -70,14 +70,19 @@ lemma comp_assoc_middle: "(\<And>x. f2 (f1 x) = x) \<Longrightarrow> f1 \<circ> 
 lemma typedef_Rep_comp: "type_definition Rep Abs UNIV \<Longrightarrow> Rep ((Abs \<circ> f \<circ> Rep) x) = f (Rep x)"
   unfolding comp_def type_definition.Abs_inverse[OF _ UNIV_I] ..
 
+definition "Sb_FTerm_pre \<equiv> \<lambda>(f1::'v::var \<Rightarrow> 'v) (f2::'tv::var \<Rightarrow> 'tv FType). (Abs_FTerm_pre :: _ \<Rightarrow> ('tv, 'v, 'btv::var, 'bv::var, 'c, 'd) FTerm_pre) \<circ> (map_sum (id f1) (map_sum id (BMV_Fixpoint.sum2.sum2.sum.Sb_0 f2) \<circ> id) \<circ> id) \<circ> Rep_FTerm_pre"
+definition "Vrs1_FTerm_pre \<equiv> \<lambda>x. \<Union>x\<in>Basic_BNFs.setl (Rep_FTerm_pre x). {x}"
+definition "Vrs2_FTerm_pre \<equiv> \<lambda>x. \<Union>x\<in>Basic_BNFs.setr (Rep_FTerm_pre x). \<Union> (BMV_Fixpoint.sum2.sum2.sum.Vrs_0_0_0 ` Basic_BNFs.setr x)"
+
 (* Transfer pbmv structure of pre-datatype to sealed version *)
 pbmv_monad "('tv::var, 'v::var, 'btv::var, 'bv::var, 'c, 'd) FTerm_pre" and "'v::var" and "'tv::var FType"
-  Sbs: "\<lambda>(f1::'v::var \<Rightarrow> 'v) (f2::'tv::var \<Rightarrow> 'tv FType). (Abs_FTerm_pre :: _ \<Rightarrow> ('tv, 'v, 'btv::var, 'bv::var, 'c, 'd) FTerm_pre) \<circ> (map_sum (id f1) (map_sum id (BMV_Fixpoint.sum2.sum2.sum.Sb_0 f2) \<circ> id) \<circ> id) \<circ> Rep_FTerm_pre" and "id :: ('v \<Rightarrow> 'v) \<Rightarrow> 'v \<Rightarrow> 'v" and "tvsubst_FType :: ('tv::var \<Rightarrow> 'tv FType) \<Rightarrow> 'tv FType \<Rightarrow> 'tv FType"
+  Sbs: "Sb_FTerm_pre :: _ \<Rightarrow> _ \<Rightarrow> _ \<Rightarrow> ('tv::var, 'v::var, 'btv::var, 'bv::var, 'c, 'd) FTerm_pre" and "id :: ('v \<Rightarrow> 'v) \<Rightarrow> 'v \<Rightarrow> 'v" and "tvsubst_FType :: ('tv::var \<Rightarrow> 'tv FType) \<Rightarrow> 'tv FType \<Rightarrow> 'tv FType"
   Injs: "id :: 'v::var \<Rightarrow> 'v" "TyVar :: 'tv::var \<Rightarrow> 'tv FType" and "id :: 'v::var \<Rightarrow> 'v" and "TyVar :: 'tv::var \<Rightarrow> 'tv FType"
-  Vrs: "\<lambda>x. \<Union>x\<in>Basic_BNFs.setl (Rep_FTerm_pre x). {x}", "\<lambda>x. \<Union>x\<in>Basic_BNFs.setr (Rep_FTerm_pre x). \<Union> (BMV_Fixpoint.sum2.sum2.sum.Vrs_0_0_0 ` Basic_BNFs.setr x)" and "\<lambda>(x::'v). {x}" and "Vrs_FType_1 :: _ \<Rightarrow> 'tv::var set"
+  Vrs: "Vrs1_FTerm_pre :: ('tv::var, 'v::var, 'btv::var, 'bv::var, 'c, 'd) FTerm_pre \<Rightarrow> _", "Vrs2_FTerm_pre :: ('tv::var, 'v::var, 'btv::var, 'bv::var, 'c, 'd) FTerm_pre \<Rightarrow> _" and "\<lambda>(x::'v). {x}" and "Vrs_FType_1 :: _ \<Rightarrow> 'tv::var set"
   Map: "\<lambda>(f1::'c \<Rightarrow> 'c') (f2::'d \<Rightarrow> 'd'). map_FTerm_pre id id id id f1 f2"
   Supps: "set5_FTerm_pre :: _ \<Rightarrow> 'c set" "set6_FTerm_pre :: _ \<Rightarrow> 'd set"
   bd: natLeq
+  apply (unfold Sb_FTerm_pre_def Vrs1_FTerm_pre_def Vrs2_FTerm_pre_def)
   subgoal
     apply (tactic \<open>resolve_tac @{context} [BMV_Monad_Def.bd_infinite_regular_card_order_of_bmv_monad bmv] 1\<close>)
     done
@@ -201,5 +206,1219 @@ pbmv_monad "('tv::var, 'v::var, 'btv::var, 'bv::var, 'c, 'd) FTerm_pre" and "'v:
   apply (tactic \<open>resolve_tac @{context} (map #Sb_cong axioms) 1\<close>; assumption)
   done
 print_pbmv_monads
+
+lemma set1_Vrs: "set1_FTerm_pre x = Vrs2_FTerm_pre x"
+  apply (unfold set1_FTerm_pre_def Vrs2_FTerm_pre_def sum.set_map UN_empty2 Un_empty_left
+    prod.set_map Un_empty_right comp_def bmv_defs
+  )
+  apply (rule refl)
+  done
+lemma set2_Vrs: "set2_FTerm_pre x = Vrs1_FTerm_pre x"
+  apply (unfold set2_FTerm_pre_def Vrs1_FTerm_pre_def sum.set_map UN_empty2 Un_empty_left
+    prod.set_map Un_empty_right comp_def bmv_defs
+  )
+  apply (rule refl)
+  done
+lemma set3_Sb: "set3_FTerm_pre (Sb_FTerm_pre f1 f2 x) = set3_FTerm_pre x"
+  apply (unfold Sb_FTerm_pre_def bmv_defs comp_def id_apply set3_FTerm_pre_def
+    prod.set_map sum.set_map UN_empty2 Un_empty_left Un_empty_right
+    Abs_FTerm_pre_inverse[OF UNIV_I] UN_simps(10)
+  )
+  apply (rule refl)
+  done
+lemma set4_Sb: "set4_FTerm_pre (Sb_FTerm_pre f1 f2 x) = set4_FTerm_pre x"
+  apply (unfold Sb_FTerm_pre_def bmv_defs comp_def id_apply set4_FTerm_pre_def
+    prod.set_map sum.set_map UN_empty2 Un_empty_left Un_empty_right
+    Abs_FTerm_pre_inverse[OF UNIV_I] UN_simps(10)
+  )
+  apply (rule refl)
+  done
+
+lemma permute_Sb_FType:
+  fixes f::"'tv::var \<Rightarrow> 'tv"
+  assumes "bij f" "|supp f| <o |UNIV::'tv set|" "|SSupp_FType g| <o |UNIV::'tv set|"
+  shows "Sb_FType (permute_FType f \<circ> g \<circ> inv f) = permute_FType f \<circ> Sb_FType g \<circ> permute_FType (inv f)"
+  apply (rule ext)
+  apply (rule trans[OF _ comp_apply[symmetric]])
+  subgoal for x
+    apply (subgoal_tac "|SSupp_FType (permute_FType f \<circ> g \<circ> inv f)| <o |UNIV|")
+     prefer 2
+     apply (subst FType.SSupp_natural)
+    apply (rule assms ordLeq_ordLess_trans[OF card_of_image])+
+    apply (binder_induction x avoiding: "IImsupp_FType (permute_FType f \<circ> g \<circ> inv f)" rule: FType.strong_induct)
+       apply (unfold IImsupp_FType_def)[1]
+       apply (rule FType.Un_bound)
+        apply (subst FType.SSupp_natural)
+          apply (rule assms)+
+        apply (rule ordLeq_ordLess_trans[OF card_of_image])
+        apply (rule assms)
+    apply (rule FType.UN_bound)
+        apply (subst FType.SSupp_natural)
+          apply (rule assms)+
+        apply (rule ordLeq_ordLess_trans[OF card_of_image])
+        apply (rule assms)
+       apply (unfold comp_def)[1]
+       apply (rule FType.set_bd_UNIV)
+
+    apply (rule trans)
+       apply (rule FType.subst)
+       apply assumption
+      apply (unfold comp_def)[1]
+      apply (rule arg_cong[of _ _ "permute_FType _"])
+      apply (rule sym)
+      apply (rule trans)
+       apply (subst FType.permute)
+    apply (rule assms bij_imp_bij_inv supp_inv_bound)+
+       apply (rule FType.subst)
+       apply (rule assms)
+      apply (rule refl)
+
+     apply (rule trans)
+      apply (rule FType.subst)
+      apply assumption
+     apply (subst FType.permute)
+       apply (rule assms bij_imp_bij_inv supp_inv_bound)+
+    apply (unfold comp_def)[1]
+     apply (subst FType.subst)
+      apply (rule assms)
+     apply (subst FType.permute)
+       apply (rule assms)+
+     apply (rule arg_cong2[of _ _ _ _ TyApp])
+      apply assumption+
+
+     apply (rule trans)
+     apply (rule FType.subst)
+      apply assumption+
+    apply (subst FType.permute)
+       apply (rule assms bij_imp_bij_inv supp_inv_bound)+
+    apply (rule trans[OF _ comp_apply[symmetric]])
+    apply (subst FType.subst)
+      apply (rule assms)
+     apply (subst (asm) FType.IImsupp_natural)
+       apply (rule assms)+
+     apply (subst (asm) image_in_bij_eq)
+      apply (rule assms)
+     apply assumption
+    apply (subst FType.permute)
+      apply (rule assms)+
+    apply (subst inv_simp2[of f])
+     apply (rule assms)
+    apply (rule arg_cong2[of _ _ _ _ TyAll])
+     apply (rule refl)
+    apply (unfold comp_def)
+    apply assumption
+    done
+  done
+
+lemma Map_Sb':
+  fixes f1::"'x1::var \<Rightarrow> 'x1" and f2::"'x2::var \<Rightarrow> 'x2" and f3::"'x3::var \<Rightarrow> 'x3" and f4::"'x4::var \<Rightarrow> 'x4"
+  assumes "bij f1" "|supp f1| <o |UNIV::'x1 set|" "bij f2" "|supp f2| <o |UNIV::'x2 set|" "|{a. g2 a \<noteq> Inj_FType_1 a}| <o |UNIV::'x1 set|"
+  shows "map_FTerm_pre f1 f2 f3 f4 f5 f6 \<circ> Sb_FTerm_pre g1 g2 = Sb_FTerm_pre (f2 \<circ> g1 \<circ> inv f2) (permute_FType f1 \<circ> g2 \<circ> inv f1) \<circ> map_FTerm_pre f1 f2 f3 f4 f5 f6"
+  apply (rule ext)
+  apply (subgoal_tac "|SSupp_FType g2| <o |UNIV::'x1 set|")
+   prefer 2
+   apply (unfold SSupp_FType_def tvVVr_tvsubst_FType_def tv\<eta>_FType_tvsubst_FType_def comp_def TyVar_def[symmetric])[1]
+  apply (rule assms)
+  apply (tactic \<open>Local_Defs.unfold0_tac @{context} @{thms
+    comp_apply map_FTerm_pre_def bmv_defs Sb_FTerm_pre_def Abs_FTerm_pre_inverse[OF UNIV_I] o_id id_apply
+    sum.map_comp prod.map_comp
+  }\<close>)
+  apply (subst permute_Sb_FType, (rule assms | assumption)+)+
+  apply (unfold comp_def)
+  apply (unfold sum.map_comp id_apply prod.map_comp comp_def)
+  apply (subst inv_simp1, rule assms)+
+  apply (subst FType.vvsubst_permute FType.permute_comp inv_o_simp1, (rule assms bij_imp_bij_inv supp_inv_bound)+)+
+  apply (unfold FType.permute_id)
+  apply (rule refl)
+  done
+
+ML \<open>
+val bmv = the (BMV_Monad_Def.pbmv_monad_of @{context} "BMV_Fixpoint.FTerm_pre")
+val axioms = BMV_Monad_Def.axioms_of_bmv_monad bmv
+val laxioms = hd axioms
+val param = the (hd (BMV_Monad_Def.params_of_bmv_monad bmv))
+\<close>
+
+(* Substitution axioms *)
+abbreviation \<eta> :: "'v::var \<Rightarrow> ('tv::var, 'v::var, 'a::var, 'b::var, 'c, 'd) FTerm_pre" where
+  "\<eta> a \<equiv> Abs_FTerm_pre (Inl a)"
+
+lemma eta_free: "set2_FTerm_pre (\<eta> a) = {a}"
+  apply (unfold set2_FTerm_pre_def sum.set_map UN_empty2 Un_empty_left Un_empty_right prod.set_map comp_def
+    Abs_FTerm_pre_inverse[OF UNIV_I] sum_set_simps UN_empty UN_single
+  )
+  apply (rule refl)
+  done
+lemma eta_inj: "\<eta> a = \<eta> b \<Longrightarrow> a = b"
+  apply (unfold Abs_FTerm_pre_inject[OF UNIV_I UNIV_I] sum.inject)
+  apply assumption
+  done
+lemma eta_natural:
+  fixes f1::"'x1::var \<Rightarrow> 'x1" and f2::"'x2::var \<Rightarrow> 'x2" and f3::"'x3::var \<Rightarrow> 'x3" and f4::"'x4::var \<Rightarrow> 'x4"
+  assumes "|supp f1| <o |UNIV::'x1 set|" "|supp f2| <o |UNIV::'x2 set|"
+    "bij f3" "|supp f3| <o |UNIV::'x3 set|" "bij f4" "|supp f4| <o |UNIV::'x4 set|"
+  shows "map_FTerm_pre f1 f2 f3 f4 f5 f6 \<circ> \<eta> = \<eta> \<circ> f2"
+  apply (rule ext)
+  apply (unfold comp_def map_FTerm_pre_def Abs_FTerm_pre_inverse[OF UNIV_I] map_sum.simps)
+  apply (rule refl)
+  done
+
+(* Construction of substitution *)
+type_synonym ('tv, 'v) P = "('v \<Rightarrow> ('tv, 'v) FTerm) \<times> ('tv \<Rightarrow> 'tv FType)"
+
+definition VVr :: "'v::var \<Rightarrow> ('tv::var, 'v) FTerm" where
+  "VVr \<equiv> FTerm_ctor \<circ> \<eta>"
+definition isVVr :: "('tv::var, 'v::var) FTerm \<Rightarrow> bool" where
+  "isVVr x \<equiv> \<exists>a. x = VVr a"
+definition asVVr :: "('tv::var, 'v::var) FTerm \<Rightarrow> 'v" where
+  "asVVr x \<equiv> (if isVVr x then SOME a. x = VVr a else undefined)"
+
+definition SSupp_FTerm :: "('v \<Rightarrow> ('tv::var, 'v::var) FTerm) \<Rightarrow> 'v set" where
+  "SSupp_FTerm f \<equiv> { a. f a \<noteq> VVr a }"
+definition IImsupp_FTerm1 :: "('v \<Rightarrow> ('tv::var, 'v::var) FTerm) \<Rightarrow> 'tv set" where
+  "IImsupp_FTerm1 f \<equiv> \<Union>(FTVars ` f ` SSupp_FTerm f)"
+definition IImsupp_FTerm2 :: "('v \<Rightarrow> ('tv::var, 'v::var) FTerm) \<Rightarrow> 'v set" where
+  "IImsupp_FTerm2 f \<equiv> SSupp_FTerm f \<union> \<Union>(FVars ` f ` SSupp_FTerm f)"
+
+definition Uctor :: "('tv::var, 'v::var, 'tv, 'v, ('tv, 'v) FTerm \<times> (('tv, 'v) P \<Rightarrow> ('tv, 'v) FTerm), ('tv, 'v) FTerm \<times> (('tv, 'v) P \<Rightarrow> ('tv, 'v) FTerm)) FTerm_pre
+  \<Rightarrow> ('tv, 'v) P \<Rightarrow> ('tv, 'v) FTerm" where
+  "Uctor y p \<equiv> case p of (f1, f2) \<Rightarrow> if isVVr (FTerm_ctor (map_FTerm_pre id id id id fst fst y)) then
+    f1 (asVVr (FTerm_ctor (map_FTerm_pre id id id id fst fst y)))
+  else
+    FTerm_ctor (Sb_FTerm_pre id f2 (map_FTerm_pre id id id id ((\<lambda>R. R (f1, f2)) \<circ> snd) ((\<lambda>R. R (f1, f2)) \<circ> snd) y))"
+
+definition PFVars_1 :: "('tv::var, 'v::var) P \<Rightarrow> 'tv set" where
+  "PFVars_1 p \<equiv> case p of (f1, f2) \<Rightarrow> IImsupp_FTerm1 f1 \<union> IImsupp_FType f2"
+definition PFVars_2 :: "('tv::var, 'v::var) P \<Rightarrow> 'v set" where
+  "PFVars_2 p \<equiv> case p of (f1, _) \<Rightarrow> IImsupp_FTerm2 f1"
+
+definition compSS_FType :: "('tv \<Rightarrow> 'tv) \<Rightarrow> ('tv \<Rightarrow> 'tv::var FType) \<Rightarrow> 'tv \<Rightarrow> 'tv FType" where
+  "compSS_FType g f \<equiv> permute_FType g \<circ> f \<circ> inv g"
+definition compSS_FTerm :: "('tv \<Rightarrow> 'tv) \<Rightarrow> ('v \<Rightarrow> 'v) \<Rightarrow> ('v \<Rightarrow> ('tv::var, 'v::var) FTerm) \<Rightarrow> 'v \<Rightarrow> ('tv, 'v) FTerm" where
+  "compSS_FTerm g1 g2 f \<equiv> permute_FTerm g1 g2 \<circ> f \<circ> inv g2"
+definition Pmap :: "('tv \<Rightarrow> 'tv) \<Rightarrow> ('v \<Rightarrow> 'v) \<Rightarrow> ('tv::var, 'v::var) P \<Rightarrow> ('tv, 'v) P" where
+  "Pmap g1 g2 p \<equiv> case p of (f1, f2) \<Rightarrow> (compSS_FTerm g1 g2 f1, compSS_FType g1 f2)"
+lemmas compSS_defs = compSS_FType_def compSS_FTerm_def
+
+definition valid_P :: "('tv::var, 'v::var) P \<Rightarrow> bool" where
+  "valid_P p \<equiv> case p of (f1, f2) \<Rightarrow>
+    |SSupp_FTerm f1| <o cmin |UNIV::'tv set| |UNIV::'v set|
+  \<and> |SSupp_FType f2| <o cmin |UNIV::'tv set| |UNIV::'v set|"
+
+lemma asVVr_VVr: "asVVr (VVr a) = a"
+  apply (unfold asVVr_def isVVr_def)
+  apply (subst if_P)
+   apply (rule exI)
+   apply (rule refl)
+  apply (rule someI2)
+   apply (rule refl)
+  apply (unfold VVr_def comp_def)
+  apply (unfold FTerm.TT_inject0)
+  apply (erule exE conjE)+
+  apply (unfold map_FTerm_pre_def comp_def Abs_FTerm_pre_inverse[OF UNIV_I]
+    map_sum.simps Abs_FTerm_pre_inject[OF UNIV_I UNIV_I] id_apply
+    sum.inject
+  )
+  apply (erule sym)
+  done
+
+ML \<open>
+val Map_Sb' = Local_Defs.unfold0 @{context} @{thms comp_apply} (#Map_Sb param RS fun_cong) RS sym
+val Vrs_Sb = maps (map_filter I) (#Vrs_Sbs laxioms);
+val Vrs_Injs = maps (maps (map_filter I) o #Vrs_Injs) axioms;
+\<close>
+
+lemma permute_VVr:
+  fixes f1::"'var::var \<Rightarrow> 'var" and f2::"'tyvar::var \<Rightarrow> 'tyvar"
+  assumes f_prems: "bij f1" "|supp f1| <o |UNIV::'var set|" "bij f2" "|supp f2| <o |UNIV::'tyvar set|"
+  shows "permute_FTerm f1 f2 (VVr a) = VVr (f2 a)"
+  apply (unfold VVr_def comp_def)
+  apply (rule trans)
+   apply (rule FTerm.permute_ctor[OF assms])
+  apply (subst fun_cong[OF eta_natural, unfolded comp_def])
+      apply (rule assms)+
+  apply (rule refl)
+  done
+
+lemma isVVr_permute:
+  fixes f1::"'var::var \<Rightarrow> 'var" and f2::"'tyvar::var \<Rightarrow> 'tyvar"
+  assumes f_prems: "bij f1" "|supp f1| <o |UNIV::'var set|" "bij f2" "|supp f2| <o |UNIV::'tyvar set|"
+  shows "isVVr (permute_FTerm f1 f2 x) = isVVr x"
+  apply (unfold isVVr_def)
+  apply (rule iffI)
+   apply (erule exE)
+   apply (drule arg_cong[of _ _ "permute_FTerm (inv f1) (inv f2)"])
+   apply (subst (asm) FTerm.permute_comp)
+           apply (rule assms bij_imp_bij_inv supp_inv_bound)+
+   apply (subst (asm) inv_o_simp1, rule assms)+
+   apply (unfold FTerm.permute_id)
+   apply hypsubst_thin
+   apply (subst permute_VVr)
+       apply (rule assms bij_imp_bij_inv supp_inv_bound)+
+   apply (rule exI)
+   apply (rule refl)
+  apply (erule exE)
+  apply hypsubst_thin
+  apply (subst permute_VVr)
+      apply (rule assms bij_imp_bij_inv supp_inv_bound)+
+  apply (rule exI)
+  apply (rule refl)
+  done
+
+lemma compSS_id0s:
+  "compSS_FType id = id"
+  "compSS_FTerm id id = id"
+  apply (unfold compSS_FType_def compSS_FTerm_def FTerm.permute_id0 FType.permute_id0 id_o o_id inv_id)
+  apply (unfold id_def)
+  apply (rule refl)+
+  done
+
+lemma compSS_comp0_FTerm:
+  fixes f1 g1::"'tyvar::var \<Rightarrow> 'tyvar" and f2 g2::"'var::var \<Rightarrow> 'var"
+  assumes g_prems: "bij g1" "|supp g1| <o cmin |UNIV::'tyvar set| |UNIV::'var set|" "bij g2" "|supp g2| <o cmin |UNIV::'tyvar set| |UNIV::'var set|"
+    and f_prems: "bij f1" "|supp f1| <o cmin |UNIV::'tyvar set| |UNIV::'var set|" "bij f2" "|supp f2| <o cmin |UNIV::'tyvar set| |UNIV::'var set|"
+  shows
+    "compSS_FTerm f1 f2 \<circ> compSS_FTerm g1 g2 = compSS_FTerm (f1 \<circ> g1) (f2 \<circ> g2)"
+  apply (unfold compSS_FTerm_def)
+  apply (subst o_inv_distrib FTerm.permute_comp0[symmetric], (rule supp_id_bound bij_id assms ordLess_ordLeq_trans cmin2 cmin1 card_of_Card_order)+)+
+  apply (rule ext)
+  apply (rule trans[OF comp_apply])
+  apply (unfold comp_assoc)
+  apply (rule refl)
+  done
+lemmas compSS_comp0s = FType.compSS_comp0[unfolded tvcompSS_tvsubst_FType_def compSS_FType_def[symmetric]] compSS_comp0_FTerm
+
+lemma IImsupp_VVrs: "f2 a \<noteq> a \<Longrightarrow> imsupp f2 \<inter> IImsupp_FTerm2 y = {} \<Longrightarrow> y a = VVr a"
+  apply (unfold imsupp_def supp_def IImsupp_FTerm2_def SSupp_FTerm_def)
+  apply (drule iffD1[OF disjoint_iff])
+  apply (erule allE)
+  apply (erule impE)
+   apply (rule UnI1)
+   apply (erule iffD2[OF mem_Collect_eq])
+  apply (unfold Un_iff de_Morgan_disj mem_Collect_eq not_not)
+  apply (erule conjE)
+  apply assumption
+  done
+
+lemma IImsupp_permute_commute:
+  fixes f1::"'var::var \<Rightarrow> 'var" and f2::"'tyvar::var \<Rightarrow> 'tyvar"
+  assumes f_prems: "bij f1" "|supp f1| <o |UNIV::'var set|" "bij f2" "|supp f2| <o |UNIV::'tyvar set|"
+  shows "imsupp f1 \<inter> IImsupp_FTerm1 y = {} \<Longrightarrow> imsupp f2 \<inter> IImsupp_FTerm2 y = {} \<Longrightarrow> permute_FTerm f1 f2 \<circ> y = y \<circ> f2"
+  apply (rule ext)
+  apply (unfold comp_def)
+  subgoal for a
+    apply (rule case_split[of "f2 a = a"])
+     apply (rule case_split[of "y a = VVr a"])
+      apply (rule trans)
+       apply (rule arg_cong[of _ _ "permute_FTerm f1 f2"])
+       apply assumption
+      apply (rule trans)
+       apply (rule permute_VVr)
+          apply (rule assms)+
+      apply (rule trans)
+       apply (rule arg_cong[of _ _ VVr])
+       apply assumption
+      apply (rule sym)
+      apply (rotate_tac -2)
+      apply (erule subst[OF sym])
+      apply assumption
+
+     apply (rule trans)
+      apply (rule FTerm.permute_cong_id)
+           apply (rule assms)+
+      (* REPEAT_DETERM *)
+       apply (erule id_onD[rotated])
+       apply (rule imsupp_id_on)
+       apply (erule Int_subset_empty2)
+       apply (unfold IImsupp_FTerm1_def SSupp_FTerm_def)[1]
+       apply (rule subsetI)
+       apply (rule UnI2)?
+       apply (rule UN_I[rotated])
+        apply assumption
+       apply (rule imageI)
+       apply (rule CollectI)
+       apply assumption
+      (* repeated *)
+      (* REPEAT_DETERM *)
+      apply (erule id_onD[rotated])
+      apply (rule imsupp_id_on)
+      apply (erule Int_subset_empty2)
+      apply (unfold IImsupp_FTerm2_def SSupp_FTerm_def)[1]
+      apply (rule subsetI)
+      apply (rule UnI2)?
+      apply (rule UN_I[rotated])
+       apply assumption
+      apply (rule imageI)
+      apply (rule CollectI)
+      apply assumption
+      (* END REPEAT_DETERM *)
+     apply (rotate_tac -2)
+     apply (erule subst[OF sym])
+     apply (rule refl)
+
+    apply (rule trans)
+     apply (rule arg_cong[of _ _ "permute_FTerm f1 f2"])
+     defer
+     apply (rule trans)
+      prefer 3
+      apply (erule IImsupp_VVrs)
+      apply assumption
+     apply (rule permute_VVr)
+        apply (rule f_prems)+
+    apply (rule sym)
+    apply (rule IImsupp_VVrs)
+     apply (erule bij_not_eq_twice[rotated])
+     apply (rule f_prems)
+    apply assumption
+    done
+  done
+
+lemma compSS_cong_id_FTerm:
+  fixes f1 g1::"'tyvar::var \<Rightarrow> 'tyvar" and f2 g2::"'var::var \<Rightarrow> 'var"
+  assumes g_prems: "bij g1" "|supp g1| <o cmin |UNIV::'tyvar set| |UNIV::'var set|" "bij g2" "|supp g2| <o cmin |UNIV::'tyvar set| |UNIV::'var set|"
+    and f_prems: "bij f1" "|supp f1| <o cmin |UNIV::'tyvar set| |UNIV::'var set|" "bij f2" "|supp f2| <o cmin |UNIV::'tyvar set| |UNIV::'var set|"
+  shows
+    "(\<And>a. a \<in> IImsupp_FTerm1 h \<Longrightarrow> f1 a = a) \<Longrightarrow> (\<And>a. a \<in> IImsupp_FTerm2 h \<Longrightarrow> f2 a = a) \<Longrightarrow> compSS_FTerm f1 f2 h = h"
+  apply (unfold compSS_FTerm_def)
+  subgoal premises prems
+    apply (subst IImsupp_permute_commute)
+          apply (rule assms cmin1 cmin2 card_of_Card_order ordLess_ordLeq_trans)+
+    (* REPEAT_DETERM *)
+      apply (rule trans[OF Int_commute])
+      apply (rule disjointI)
+      apply (drule prems)
+      apply (erule bij_id_imsupp[rotated])
+      apply (rule assms)
+    (* repeated *)
+      apply (rule trans[OF Int_commute])
+      apply (rule disjointI)
+      apply (drule prems)
+      apply (erule bij_id_imsupp[rotated])
+      apply (rule assms)
+    (* END REPEAT_DETERM *)
+    apply (unfold comp_assoc)
+    apply (subst inv_o_simp2)
+     apply (rule assms)
+    apply (rule o_id)
+    done
+  done
+lemmas compSS_cong_ids = FType.compSS_cong_id[unfolded tvcompSS_tvsubst_FType_def compSS_FType_def[symmetric]] compSS_cong_id_FTerm
+
+lemma SSupp_natural_FTerm:
+  fixes f1::"'tyvar::var \<Rightarrow> 'tyvar" and f2::"'var::var \<Rightarrow> 'var"
+  assumes f_prems: "bij f1" "|supp f1| <o |UNIV::'tyvar set|" "bij f2" "|supp f2| <o |UNIV::'var set|"
+  shows
+    "SSupp_FTerm (permute_FTerm f1 f2 \<circ> y \<circ> inv f2) = f2 ` SSupp_FTerm y"
+  apply (unfold SSupp_FTerm_def)
+  apply (rule set_eqI)
+  apply (rule iffI)
+   apply (unfold mem_Collect_eq comp_def VVr_def image_Collect)
+   apply (erule contrapos_np)
+   apply (drule Meson.not_exD)
+   apply (erule allE)
+   apply (drule iffD1[OF de_Morgan_conj])
+   apply (erule disjE)
+    apply (subst (asm) inv_simp2[of f2])
+     apply (rule assms)
+    apply (erule notE)
+    apply (rule refl)
+   apply (drule notnotD)
+   apply (drule sym)
+   apply (erule subst)
+   apply (rule trans)
+    apply (rule FTerm.permute_ctor)
+       apply (rule assms)+
+   apply (subst fun_cong[OF eta_natural, unfolded comp_def])
+       apply (rule assms)+
+   apply (subst inv_simp2[of f2])
+    apply (rule f_prems)
+   apply (rule refl)
+  apply (erule exE)
+  apply (erule conjE)
+  apply hypsubst
+  apply (subst inv_simp1)
+   apply (rule f_prems)
+  apply (erule contrapos_nn)
+  apply (drule arg_cong[of _ _ "permute_FTerm (inv f1) (inv f2)"])
+  apply (subst (asm) FTerm.permute_comp)
+          apply (rule assms supp_inv_bound bij_imp_bij_inv)+
+  apply (subst (asm) inv_o_simp1, rule assms)+
+  apply (unfold FTerm.permute_id)
+  apply (erule trans)
+  apply (rule trans)
+   apply (rule FTerm.permute_ctor)
+      apply (rule assms supp_inv_bound bij_imp_bij_inv)+
+  apply (subst fun_cong[OF eta_natural, unfolded comp_def])
+      apply (rule assms supp_inv_bound bij_imp_bij_inv)+
+  apply (subst inv_simp1)
+   apply (rule assms)
+  apply (rule refl)
+  done
+lemmas SSupp_naturals = FType.SSupp_natural SSupp_natural_FTerm
+
+lemma IImsupp_natural_FTerm:
+  fixes f1::"'tyvar::var \<Rightarrow> 'tyvar" and f2::"'var::var \<Rightarrow> 'var"
+  assumes f_prems: "bij f1" "|supp f1| <o |UNIV::'tyvar set|" "bij f2" "|supp f2| <o |UNIV::'var set|"
+  shows
+    "IImsupp_FTerm1 (permute_FTerm f1 f2 \<circ> y \<circ> inv f2) = f1 ` IImsupp_FTerm1 y"
+    "IImsupp_FTerm2 (permute_FTerm f1 f2 \<circ> y \<circ> inv f2) = f2 ` IImsupp_FTerm2 y"
+   apply (unfold IImsupp_FTerm1_def IImsupp_FTerm2_def image_UN image_Un)
+   apply (rule arg_cong2[of _ _ _ _ "(\<union>)"])?
+   apply (subst SSupp_naturals)
+       apply (rule assms)+
+   apply (unfold image_comp comp_assoc)[1]
+   apply (subst inv_o_simp1, rule assms)
+   apply (unfold o_id)
+   apply (unfold comp_def)[1]
+   apply (subst FTerm.FVars_permute, (rule assms)+)
+   apply (rule refl)
+    (* repeated *)
+  apply (rule arg_cong2[of _ _ _ _ "(\<union>)"])?
+   apply (subst SSupp_naturals)
+       apply (rule assms)+
+   apply (rule refl)
+    (* repeated *)
+  apply (rule arg_cong2[of _ _ _ _ "(\<union>)"])?
+  apply (subst SSupp_naturals)
+      apply (rule assms)+
+  apply (unfold image_comp comp_assoc)[1]
+  apply (subst inv_o_simp1, rule assms)
+  apply (unfold o_id)
+  apply (unfold comp_def)[1]
+  apply (subst FTerm.FVars_permute, (rule assms)+)
+  apply (rule refl)
+  done
+lemmas IImsupp_naturals = FType.IImsupp_natural IImsupp_natural_FTerm
+
+(* Recursor axioms *)
+lemma Pmap_id0: "Pmap id id = id"
+  apply (rule ext)
+  apply (unfold Pmap_def case_prod_beta compSS_id0s)
+  apply (unfold id_def prod.collapse)
+  apply (rule refl)
+  done
+
+lemma Pmap_comp0:
+  fixes f1 g1::"'tyvar::var \<Rightarrow> 'tyvar" and f2 g2::"'var::var \<Rightarrow> 'var"
+  assumes g_prems: "bij g1" "|supp g1| <o cmin |UNIV::'tyvar set| |UNIV::'var set|" "bij g2" "|supp g2| <o cmin |UNIV::'tyvar set| |UNIV::'var set|"
+    and f_prems: "bij f1" "|supp f1| <o cmin |UNIV::'tyvar set| |UNIV::'var set|" "bij f2" "|supp f2| <o cmin |UNIV::'tyvar set| |UNIV::'var set|"
+  shows
+    "Pmap f1 f2 \<circ> Pmap g1 g2 = Pmap (f1 \<circ> g1) (f2 \<circ> g2)"
+  apply (rule ext)
+  apply (unfold Pmap_def case_prod_beta)
+  apply (rule trans[OF comp_apply])
+  apply (unfold prod.inject fst_conv snd_conv)
+  apply (rule conjI bij_id supp_id_bound assms ordLess_ordLeq_trans cmin1 card_of_Card_order
+      trans[OF comp_apply[symmetric] fun_cong[OF compSS_comp0s(1)]]
+      trans[OF comp_apply[symmetric] fun_cong[OF compSS_comp0s(2)]]
+      )+
+  done
+
+lemma valid_Pmap:
+  fixes f1::"'tyvar::var \<Rightarrow> 'tyvar" and f2::"'var::var \<Rightarrow> 'var"
+  assumes f_prems: "bij f1" "|supp f1| <o cmin |UNIV::'tyvar set| |UNIV::'var set|" "bij f2" "|supp f2| <o cmin |UNIV::'tyvar set| |UNIV::'var set|"
+  shows "valid_P p \<Longrightarrow> valid_P (Pmap f1 f2 p)"
+  apply (unfold valid_P_def Pmap_def case_prod_beta compSS_defs fst_conv snd_conv)
+  apply (erule conj_forward)+
+   apply (subst SSupp_naturals; (assumption | rule assms cmin1 cmin2 card_of_Card_order ordLeq_ordLess_trans[OF card_of_image] ordLess_ordLeq_trans)+)+
+  done
+
+lemma PFVars_Pmaps:
+  fixes f1::"'tyvar::var \<Rightarrow> 'tyvar" and f2::"'var::var \<Rightarrow> 'var"
+  assumes f_prems: "bij f1" "|supp f1| <o cmin |UNIV::'tyvar set| |UNIV::'var set|" "bij f2" "|supp f2| <o cmin |UNIV::'tyvar set| |UNIV::'var set|"
+  shows "PFVars_1 (Pmap f1 f2 p) = f1 ` PFVars_1 p"
+    "PFVars_2 (Pmap f1 f2 p) = f2 ` PFVars_2 p"
+  subgoal
+    apply (unfold PFVars_1_def Pmap_def case_prod_beta fst_conv snd_conv compSS_defs)
+    apply (subst IImsupp_naturals, (rule assms cmin1 cmin2 card_of_Card_order ordLess_ordLeq_trans)+)+
+    apply (unfold image_Un)?
+    apply (rule refl)
+    done
+  subgoal
+    apply (unfold PFVars_2_def Pmap_def case_prod_beta fst_conv snd_conv compSS_defs)
+    apply (subst IImsupp_naturals, (rule assms cmin1 cmin2 card_of_Card_order ordLess_ordLeq_trans)+)+
+    apply (unfold image_Un)?
+    apply (rule refl)
+    done
+  done
+
+lemma Pmap_cong_id:
+  fixes f1::"'tyvar::var \<Rightarrow> 'tyvar" and f2::"'var::var \<Rightarrow> 'var"
+  assumes f_prems: "bij f1" "|supp f1| <o cmin |UNIV::'tyvar set| |UNIV::'var set|" "bij f2" "|supp f2| <o cmin |UNIV::'tyvar set| |UNIV::'var set|"
+  shows "(\<And>a. a \<in> PFVars_1 p \<Longrightarrow> f1 a = a) \<Longrightarrow> (\<And>a. a \<in> PFVars_2 p \<Longrightarrow> f2 a = a) \<Longrightarrow> Pmap f1 f2 p = p"
+  apply (unfold PFVars_1_def PFVars_2_def Pmap_def case_prod_beta)
+  subgoal premises prems
+    apply (subst compSS_cong_ids, (rule f_prems prems cmin1 cmin2 card_of_Card_order ordLess_ordLeq_trans | erule UnI2 UnI1 | rule UnI1)+)+
+    apply assumption
+    apply (unfold prod.collapse)
+    apply (rule refl)
+    done
+  done
+
+lemmas Cinfinite_UNIV = conjI[OF FTerm_pre.UNIV_cinfinite card_of_Card_order]
+lemmas Cinfinite_card = cmin_Cinfinite[OF Cinfinite_UNIV Cinfinite_UNIV]
+lemmas regularCard_card = cmin_regularCard[OF FTerm_pre.var_regular FTerm_pre.var_regular Cinfinite_UNIV Cinfinite_UNIV]
+lemmas Un_bound = regularCard_Un[OF conjunct2[OF Cinfinite_card] conjunct1[OF Cinfinite_card] regularCard_card]
+lemmas UN_bound = regularCard_UNION[OF conjunct2[OF Cinfinite_card] conjunct1[OF Cinfinite_card] regularCard_card]
+
+lemma small_PFVarss:
+  "valid_P p \<Longrightarrow> |PFVars_1 (p::('tyvar::var, 'var::var) P)| <o cmin |UNIV::'tyvar set| |UNIV::'var set|"
+  "valid_P p \<Longrightarrow> |PFVars_2 p| <o cmin |UNIV::'tyvar set| |UNIV::'var set|"
+  subgoal
+    apply (unfold PFVars_1_def case_prod_beta IImsupp_FTerm1_def IImsupp_FTerm2_def IImsupp_FType_def comp_def valid_P_def)
+    apply (erule conjE)+
+        apply (assumption | rule Un_bound UN_bound ordLeq_ordLess_trans[OF card_of_image] FType.set_bd_UNIV FTerm.FVars_bd_UNIVs cmin_greater card_of_Card_order)+
+    done
+  (* copied from above *)
+  subgoal
+    apply (unfold PFVars_2_def case_prod_beta IImsupp_FTerm1_def IImsupp_FTerm2_def IImsupp_FType_def comp_def valid_P_def)
+    apply (erule conjE)+
+        apply (assumption | rule Un_bound UN_bound ordLeq_ordLess_trans[OF card_of_image] FType.set_bd_UNIV FTerm.FVars_bd_UNIVs cmin_greater card_of_Card_order)+
+    done
+  done
+
+lemma FTVars_subset: "valid_P p \<Longrightarrow> set3_FTerm_pre y \<inter> PFVars_1 p = {} \<Longrightarrow>
+  (\<And>t pu p. valid_P p \<Longrightarrow> (t, pu) \<in> set5_FTerm_pre y \<union> set6_FTerm_pre y \<Longrightarrow> FTVars (pu p) \<subseteq> FTVars t \<union> PFVars_1 p) \<Longrightarrow>
+  FTVars (Uctor y p) \<subseteq> FTVars (FTerm_ctor (map_FTerm_pre id id id id fst fst y)) \<union> PFVars_1 p"
+  subgoal premises prems
+    apply (unfold Uctor_def case_prod_beta)
+    apply (rule case_split)
+     apply (subst if_P)
+      apply assumption
+     apply (unfold isVVr_def)[1]
+     apply (erule exE)
+     apply (drule sym)
+    apply (erule subst)
+     apply (unfold asVVr_VVr)
+     apply (rule case_split[of "_ = _"])
+      apply (rule iffD2[OF arg_cong2[OF _ refl, of _ _ "(\<subseteq>)"]])
+       apply (rule arg_cong[of _ _ FTVars])
+       apply assumption
+      apply (rule Un_upper1)
+     apply (rule subsetI)
+     apply (rule UnI2)
+     apply (unfold PFVars_1_def case_prod_beta IImsupp_FTerm1_def SSupp_FTerm_def image_comp[unfolded comp_def])[1]
+     apply (rule UnI1)
+     apply (rule UN_I)
+      apply (rule CollectI)
+      apply assumption
+     apply assumption
+    apply (unfold if_not_P)
+    apply (erule thin_rl)
+
+    apply (subgoal_tac "|{ a. id a \<noteq> id a }| <o |UNIV::'v set|")
+     prefer 2
+      apply (rule card_of_subset_bound[OF _ emp_bound])
+      apply (rule subset_emptyI)
+      apply (drule CollectD)
+      apply (rotate_tac -1)
+      apply (erule contrapos_np)
+     apply (rule refl)
+    apply (subgoal_tac "|{ a. snd p a \<noteq> TyVar a }| <o |UNIV::'tv set|")
+     prefer 2
+     apply (insert prems(1))[1]
+     apply (unfold valid_P_def case_prod_beta SSupp_FType_def tvVVr_tvsubst_FType_def tv\<eta>_FType_tvsubst_FType_def TyVar_def[symmetric] comp_def)[1]
+     apply (erule conjE)
+     apply (erule ordLess_ordLeq_trans)
+     apply (rule cmin1)
+    apply (rule card_of_Card_order)+
+
+     apply (tactic \<open>EqSubst.eqsubst_tac @{context} [0] [Map_Sb'] 1\<close>)
+       apply assumption
+    apply assumption
+    apply (unfold FTerm.FVars_ctor)
+    apply (subst FTerm_pre.set_map, (rule bij_id supp_id_bound)+)+
+    apply (unfold image_id image_comp comp_def prod.collapse)
+    apply (rule Un_mono')+
+      apply (unfold set3_Sb set4_Sb set1_Vrs set2_Vrs)
+      apply (tactic \<open>EqSubst.eqsubst_tac @{context} [0] Vrs_Sb 1\<close>)
+        apply assumption+
+      apply (unfold PFVars_1_def case_prod_beta IImsupp_FType_def SSupp_FType_def
+        tvVVr_tvsubst_FType_def tv\<eta>_FType_tvsubst_FType_def TyVar_def[symmetric] comp_def
+      )[1]
+      apply (rule subsetI)
+      apply (erule UN_E)
+    apply (rule case_split[of "_ = _", rotated])
+      apply (rule UnI2)+
+       apply (rule UN_I)
+        apply (rule CollectI)
+        apply assumption
+       apply assumption
+      apply (rule UnI1)
+      apply (rotate_tac -2)
+      apply (drule iffD1[OF arg_cong2[OF refl, of _ _ "(\<in>)"], rotated])
+       apply (erule arg_cong)
+      apply (tactic \<open>Local_Defs.unfold0_tac @{context} Vrs_Injs\<close>)
+      apply (drule singletonD)
+      apply hypsubst
+      apply assumption
+
+    apply (rule iffD2[OF arg_cong2[OF refl, of _ _ "(\<subseteq>)"]])
+      apply (rule Diff_Un_disjunct)
+      apply (rule prems)
+     apply (rule Diff_mono[OF _ subset_refl])
+     apply (unfold UN_extend_simps(2))
+    (* REPEAT_DETERM *)
+     apply (rule subset_If)
+      apply (tactic \<open>Local_Defs.unfold0_tac @{context} (#Supp_Sb param)\<close>)
+      apply (unfold UN_empty')[1]
+      apply (rule empty_subsetI)
+     apply (rule UN_mono[OF subset_refl])
+     apply (rule prems)
+      apply (rule prems)
+     apply (unfold prod.collapse)
+     apply (erule UnI2 UnI1)
+    (* repeated *)
+     apply (rule subset_If)
+      apply (tactic \<open>Local_Defs.unfold0_tac @{context} (#Supp_Sb param)\<close>)
+      apply (unfold UN_empty')[1]
+      apply (rule empty_subsetI)
+     apply (rule UN_mono[OF subset_refl])
+     apply (rule prems)
+      apply (rule prems)
+     apply (unfold prod.collapse)
+     apply (erule UnI2 UnI1)
+    (* END REPEAT_DETERM *)
+    done
+  done
+
+lemma FVars_subset: "valid_P p \<Longrightarrow> set4_FTerm_pre y \<inter> PFVars_2 p = {} \<Longrightarrow>
+  (\<And>t pu p. valid_P p \<Longrightarrow> (t, pu) \<in> set5_FTerm_pre y \<union> set6_FTerm_pre y \<Longrightarrow> FVars (pu p) \<subseteq> FVars t \<union> PFVars_2 p) \<Longrightarrow>
+  FVars (Uctor y p) \<subseteq> FVars (FTerm_ctor (map_FTerm_pre id id id id fst fst y)) \<union> PFVars_2 p"
+  subgoal premises prems
+    apply (unfold Uctor_def case_prod_beta)
+    apply (rule case_split)
+     apply (subst if_P)
+      apply assumption
+     apply (unfold isVVr_def)[1]
+     apply (erule exE)
+     apply (drule sym)
+    apply (erule subst)
+     apply (unfold asVVr_VVr)
+     apply (rule case_split[of "_ = _"])
+      apply (rule iffD2[OF arg_cong2[OF _ refl, of _ _ "(\<subseteq>)"]])
+       apply (rule arg_cong[of _ _ FVars])
+       apply assumption
+      apply (rule Un_upper1)
+     apply (rule subsetI)
+     apply (rule UnI2)
+     apply (unfold PFVars_2_def case_prod_beta IImsupp_FTerm2_def SSupp_FTerm_def image_comp[unfolded comp_def])[1]
+    apply (rule UnI2)
+     apply (rule UN_I)
+      apply (rule CollectI)
+      apply assumption
+     apply assumption
+    apply (unfold if_not_P)
+    apply (erule thin_rl)
+
+    apply (subgoal_tac "|{ a. id a \<noteq> id a }| <o |UNIV::'v set|")
+     prefer 2
+      apply (rule card_of_subset_bound[OF _ emp_bound])
+      apply (rule subset_emptyI)
+      apply (drule CollectD)
+      apply (rotate_tac -1)
+      apply (erule contrapos_np)
+     apply (rule refl)
+    apply (subgoal_tac "|{ a. snd p a \<noteq> TyVar a }| <o |UNIV::'tv set|")
+     prefer 2
+     apply (insert prems(1))[1]
+     apply (unfold valid_P_def case_prod_beta SSupp_FType_def tvVVr_tvsubst_FType_def tv\<eta>_FType_tvsubst_FType_def TyVar_def[symmetric] comp_def)[1]
+     apply (erule conjE)
+     apply (erule ordLess_ordLeq_trans)
+     apply (rule cmin1)
+    apply (rule card_of_Card_order)+
+
+     apply (tactic \<open>EqSubst.eqsubst_tac @{context} [0] [Map_Sb'] 1\<close>)
+       apply assumption
+    apply assumption
+    apply (unfold FTerm.FVars_ctor)
+    apply (subst FTerm_pre.set_map, (rule bij_id supp_id_bound)+)+
+    apply (unfold image_id image_comp comp_def prod.collapse)
+    apply (rule Un_mono')+
+      apply (unfold set3_Sb set4_Sb set1_Vrs set2_Vrs)
+      apply (tactic \<open>EqSubst.eqsubst_tac @{context} [0] Vrs_Sb 1\<close>)
+        apply assumption+
+      apply (unfold PFVars_2_def case_prod_beta IImsupp_FTerm2_def SSupp_FType_def
+        tvVVr_tvsubst_FType_def tv\<eta>_FType_tvsubst_FType_def TyVar_def[symmetric] comp_def
+      )[1]
+      apply (rule subsetI)
+      apply (erule UN_E)
+    apply (rule UnI1)
+      apply (tactic \<open>Local_Defs.unfold0_tac @{context} Vrs_Injs\<close>)
+      apply (drule singletonD)
+      apply hypsubst
+      apply assumption
+
+    apply (rule iffD2[OF arg_cong2[OF refl, of _ _ "(\<subseteq>)"]])
+      apply (rule Diff_Un_disjunct)
+      apply (rule prems)
+     apply (rule Diff_mono[OF _ subset_refl])
+     apply (unfold UN_extend_simps(2))
+    (* REPEAT_DETERM *)
+     apply (rule subset_If)
+      apply (tactic \<open>Local_Defs.unfold0_tac @{context} (#Supp_Sb param)\<close>)
+      apply (unfold UN_empty')[1]
+      apply (rule empty_subsetI)
+     apply (rule UN_mono[OF subset_refl])
+     apply (rule prems)
+      apply (rule prems)
+     apply (unfold prod.collapse)
+     apply (erule UnI2 UnI1)
+    (* repeated *)
+     apply (rule subset_If)
+      apply (tactic \<open>Local_Defs.unfold0_tac @{context} (#Supp_Sb param)\<close>)
+      apply (unfold UN_empty')[1]
+      apply (rule empty_subsetI)
+     apply (rule UN_mono[OF subset_refl])
+     apply (rule prems)
+      apply (rule prems)
+     apply (unfold prod.collapse)
+     apply (erule UnI2 UnI1)
+    (* END REPEAT_DETERM *)
+    done
+  done
+
+lemma permute_Uctor:
+  fixes f1::"'tv::var \<Rightarrow> 'tv" and f2::"'v::var \<Rightarrow> 'v"
+  shows "valid_P p \<Longrightarrow> bij f1 \<Longrightarrow> |supp f1| <o cmin |UNIV::'tv set| |UNIV::'v set| \<Longrightarrow> bij f2 \<Longrightarrow> |supp f2| <o cmin |UNIV::'tv set| |UNIV::'v set|
+  \<Longrightarrow> permute_FTerm f1 f2 (Uctor y p) = Uctor (map_FTerm_pre f1 f2 f1 f2
+    (\<lambda>(t, pu). (permute_FTerm f1 f2 t, \<lambda>p. if valid_P p then permute_FTerm f1 f2 (pu (Pmap (inv f1) (inv f2) p)) else undefined))
+    (\<lambda>(t, pu). (permute_FTerm f1 f2 t, \<lambda>p. if valid_P p then permute_FTerm f1 f2 (pu (Pmap (inv f1) (inv f2) p)) else undefined))
+  y) (Pmap f1 f2 p)"
+  apply (unfold Uctor_def)
+  apply (subst FTerm_pre.map_comp, (assumption | rule supp_id_bound bij_id ordLess_ordLeq_trans cmin1 cmin2 card_of_Card_order)+)+
+  apply (unfold id_o_commute[of f1] id_o_commute[of f2] fst_o_f comp_assoc comp_def[of snd] snd_conv case_prod_beta prod.collapse)
+  apply (subst FTerm_pre.map_comp[symmetric], (assumption | rule supp_id_bound bij_id ordLess_ordLeq_trans cmin1 cmin2 card_of_Card_order)+)+
+  apply (subst FTerm.permute_ctor[symmetric] isVVr_permute, (assumption | rule ordLess_ordLeq_trans cmin1 cmin2 card_of_Card_order)+)+
+
+  apply (rule case_split)
+   apply (subst if_P)
+    apply assumption
+   apply (unfold if_P if_not_P)
+   apply (unfold isVVr_def)[1]
+   apply (erule exE)
+   apply (erule subst[OF sym])
+   apply (subst permute_VVr)
+       apply (assumption | rule ordLess_ordLeq_trans cmin1 cmin2 card_of_Card_order)+
+   apply (unfold Pmap_def case_prod_beta fst_conv snd_conv asVVr_VVr compSS_FTerm_def comp_def)[1]
+   apply (subst inv_simp1)
+    apply assumption
+   apply (rule refl)
+
+  apply (rule trans)
+   apply (rule FTerm.permute_ctor)
+      apply (assumption | rule ordLess_ordLeq_trans cmin1 cmin2 card_of_Card_order)+
+
+  apply (subgoal_tac "|{ a. id a \<noteq> id a }| <o |UNIV::'v set|")
+   prefer 2
+   apply (rule card_of_subset_bound[OF _ emp_bound])
+   apply (rule subset_emptyI)
+   apply (drule CollectD)
+   apply (rotate_tac -1)
+   apply (erule contrapos_np)
+   apply (rule refl)
+  apply (subgoal_tac "|{ a. snd p a \<noteq> TyVar a }| <o |UNIV::'tv set|")
+   prefer 2
+   apply (unfold valid_P_def case_prod_beta SSupp_FType_def tvVVr_tvsubst_FType_def tv\<eta>_FType_tvsubst_FType_def TyVar_def[symmetric] comp_def)[1]
+   apply (erule conjE)
+   apply (erule ordLess_ordLeq_trans)
+   apply (rule cmin1)
+    apply (rule card_of_Card_order)+
+
+     apply (tactic \<open>EqSubst.eqsubst_tac @{context} [0] [Map_Sb'] 1\<close>)
+       apply assumption
+   apply assumption
+
+  apply (subst FTerm_pre.map_comp, (assumption | rule supp_id_bound bij_id ordLess_ordLeq_trans cmin1 cmin2 card_of_Card_order)+)+
+  apply (unfold id_o o_id)
+  apply (unfold comp_def)
+  apply (subst if_P inv_o_simp1 trans[OF comp_apply[symmetric] Pmap_comp0[THEN fun_cong]], (rule valid_Pmap bij_imp_bij_inv supp_inv_bound | assumption)+)+
+  apply (unfold trans[OF Pmap_id0[THEN fun_cong] id_apply])
+  apply (unfold Pmap_def case_prod_beta snd_conv compSS_FType_def)
+  apply (subst trans[OF comp_apply[symmetric] Map_Sb'[THEN fun_cong]])
+      apply (assumption | rule ordLess_ordLeq_trans cmin1 cmin2 card_of_Card_order)+
+  apply (unfold id_o o_id inv_o_simp2)
+  apply (unfold comp_def)
+  apply (rule refl)
+  done
+
+ML \<open>
+val nvars: int = 2
+
+val parameters = {
+  P = @{typ "('tv::var, 'v::var) P"},
+  Pmap = @{term "Pmap :: _ \<Rightarrow> _ \<Rightarrow> _ \<Rightarrow> ('tv::var, 'v::var) P"},
+  PFVarss = [
+    @{term "PFVars_1 :: ('tv::var, 'v::var) P \<Rightarrow> _"},
+    @{term "PFVars_2 :: ('tv::var, 'v::var) P \<Rightarrow> _"}
+  ],
+  avoiding_sets = [@{term "{} :: 'tv::var set"}, @{term "{} :: 'v::var set"}],
+  min_bound = true,
+  validity = SOME {
+    pred = @{term "valid_P :: ('tv::var, 'v::var) P \<Rightarrow> _"},
+    valid_Pmap = fn ctxt => HEADGOAL (resolve_tac ctxt @{thms valid_Pmap} THEN_ALL_NEW assume_tac ctxt)
+  },
+  axioms = {
+    Pmap_id0 = fn ctxt => EVERY1 [
+      resolve_tac ctxt [trans],
+      resolve_tac ctxt @{thms fun_cong[OF Pmap_id0]},
+      resolve_tac ctxt @{thms id_apply}
+    ],
+    Pmap_comp0 = fn ctxt => resolve_tac ctxt @{thms fun_cong[OF Pmap_comp0[symmetric]]} 1 THEN REPEAT_DETERM (assume_tac ctxt 1),
+    Pmap_cong_id = fn ctxt => resolve_tac ctxt @{thms Pmap_cong_id} 1 THEN REPEAT_DETERM (assume_tac ctxt 1 ORELSE Goal.assume_rule_tac ctxt 1),
+    PFVars_Pmaps = replicate nvars (fn ctxt => resolve_tac ctxt @{thms PFVars_Pmaps} 1 THEN REPEAT_DETERM (assume_tac ctxt 1)),
+    small_PFVarss = replicate nvars (fn ctxt => resolve_tac ctxt @{thms small_PFVarss} 1 THEN assume_tac ctxt 1),
+    small_avoiding_sets = replicate nvars (fn ctxt => HEADGOAL (resolve_tac ctxt @{thms cmin_greater}
+      THEN_ALL_NEW resolve_tac ctxt @{thms card_of_Card_order emp_bound}))
+  }
+} : (Proof.context -> tactic) MRBNF_Recursor.parameter;
+\<close>
+
+ML \<open>
+val fp_res = the (MRBNF_FP_Def_Sugar.fp_result_of @{context} "BMV_Fixpoint.FTerm")
+val quot = hd (#quotient_fps fp_res);
+val vars = map TVar (rev (Term.add_tvarsT (#T quot) []));
+\<close>
+
+ML \<open>
+val model = MRBNF_Recursor.mk_quotient_model quot (vars ~~ [@{typ "'tv::var"}, @{typ "'v::var"}]) {
+  binding = @{binding "tvsubst_FTerm"},
+  Uctor = @{term "Uctor :: _ \<Rightarrow> ('tv::var, 'v::var) P \<Rightarrow> _"},
+  validity = NONE,
+  axioms = {
+    FVars_subsets = [
+      fn ctxt => EVERY1 [
+        K (Local_Defs.unfold0_tac ctxt @{thms Un_empty_right}),
+        resolve_tac ctxt @{thms FTVars_subset},
+        REPEAT_DETERM o assume_tac ctxt,
+        Goal.assume_rule_tac ctxt
+      ],
+      fn ctxt => EVERY1 [
+        K (Local_Defs.unfold0_tac ctxt @{thms Un_empty_right}),
+        resolve_tac ctxt @{thms FVars_subset},
+        REPEAT_DETERM o assume_tac ctxt,
+        Goal.assume_rule_tac ctxt
+      ]
+    ],
+    permute_Uctor = fn ctxt => HEADGOAL (resolve_tac ctxt @{thms permute_Uctor} THEN_ALL_NEW assume_tac ctxt)
+  }
+}
+\<close>
+
+local_setup \<open>fn lthy =>
+let
+  val qualify = I
+  val (ress, lthy) = MRBNF_Recursor.create_binding_recursor qualify fp_res parameters [model] lthy
+
+  val notes =
+    [ ("rec_Uctor", map (Local_Defs.unfold0 lthy @{thms Un_empty_right} o #rec_Uctor) ress)
+    ] |> (map (fn (thmN, thms) =>
+      ((Binding.qualify true "FTerm" (Binding.name thmN), []), [(thms, [])])
+    ));
+  val (_, lthy) = Local_Theory.notes notes lthy
+  val _ = @{print} ress
+in lthy end
+\<close>
+print_theorems
+
+definition tvsubst_FTerm :: "('v \<Rightarrow> ('tv::var, 'v::var) FTerm) \<Rightarrow> ('tv \<Rightarrow> 'tv FType) \<Rightarrow> ('tv, 'v) FTerm \<Rightarrow> ('tv, 'v) FTerm" where
+  "tvsubst_FTerm f1 f2 t \<equiv> ff0_tvsubst_FTerm t (f1, f2)"
+
+type_synonym ('tv, 'v) U1_pre = "('tv, 'v, 'tv, 'v, ('tv, 'v) FTerm, ('tv, 'v) FTerm) FTerm_pre"
+
+lemmas eta_natural' = fun_cong[OF eta_natural, unfolded comp_def]
+
+lemma eta_set_empties:
+  fixes a::"'v::var"
+  shows
+    "set1_FTerm_pre (\<eta> a :: ('tv::var, 'v) U1_pre) = {}"
+    "set3_FTerm_pre (\<eta> a :: ('tv::var, 'v) U1_pre) = {}"
+    "set4_FTerm_pre (\<eta> a :: ('tv::var, 'v) U1_pre) = {}"
+    "set5_FTerm_pre (\<eta> a :: ('tv::var, 'v) U1_pre) = {}"
+    "set6_FTerm_pre (\<eta> a :: ('tv::var, 'v) U1_pre) = {}"
+      apply -
+  subgoal
+    apply (rule set_eqI)
+    apply (unfold empty_iff)
+    apply (rule iffI)
+     apply (rule exE[OF exists_fresh, of "set1_FTerm_pre (\<eta> a)"])
+      apply (rule FTerm_pre.set_bd_UNIV)
+     apply (drule iffD1[OF arg_cong2[OF refl, of _ _ "(\<in>)"], rotated])
+      apply (rule arg_cong[of _ _ set1_FTerm_pre])
+      prefer 2
+      apply (subst (asm) FTerm_pre.set_map)
+            prefer 7
+            apply (erule swap_fresh)
+            apply assumption
+           apply (rule supp_id_bound bij_id supp_swap_bound bij_swap infinite_UNIV)+
+     apply (rule sym)
+     apply (rule trans)
+      apply (rule fun_cong[OF eta_natural, unfolded comp_def])
+           apply (rule supp_id_bound bij_id supp_swap_bound bij_swap infinite_UNIV)+
+     apply (unfold id_def)
+     apply (rule refl)
+    apply (erule FalseE)
+    done
+  subgoal
+    apply (rule set_eqI)
+    apply (unfold empty_iff)
+    apply (rule iffI)
+     apply (rule exE[OF exists_fresh, of "set3_FTerm_pre (\<eta> a)"])
+      apply (rule FTerm_pre.set_bd_UNIV)
+     apply (drule iffD1[OF arg_cong2[OF refl, of _ _ "(\<in>)"], rotated])
+      apply (rule arg_cong[of _ _ set3_FTerm_pre])
+      prefer 2
+      apply (subst (asm) FTerm_pre.set_map)
+            prefer 7
+            apply (erule swap_fresh)
+            apply assumption
+           apply (rule supp_id_bound bij_id supp_swap_bound bij_swap infinite_UNIV)+
+     apply (rule sym)
+     apply (rule trans)
+      apply (rule fun_cong[OF eta_natural, unfolded comp_def])
+           apply (rule supp_id_bound bij_id supp_swap_bound bij_swap infinite_UNIV)+
+     apply (unfold id_def)
+     apply (rule refl)
+    apply (erule FalseE)
+    done
+  subgoal
+    apply (rule set_eqI)
+    apply (unfold empty_iff)
+    apply (rule iffI)
+     apply (rule exE[OF exists_fresh, of "set4_FTerm_pre (\<eta> a)"])
+      apply (rule FTerm_pre.set_bd_UNIV)
+     apply (drule iffD1[OF arg_cong2[OF refl, of _ _ "(\<in>)"], rotated])
+      apply (rule arg_cong[of _ _ set4_FTerm_pre])
+      prefer 2
+      apply (subst (asm) FTerm_pre.set_map)
+            prefer 7
+            apply (erule swap_fresh)
+            apply assumption
+           apply (rule supp_id_bound bij_id supp_swap_bound bij_swap infinite_UNIV)+
+     apply (rule sym)
+     apply (rule trans)
+      apply (rule eta_natural')
+           apply (rule supp_id_bound bij_id supp_swap_bound bij_swap infinite_UNIV)+
+     apply (unfold id_def)
+     apply (rule refl)
+    apply (erule FalseE)
+    done
+  subgoal
+    apply (rule set_eqI)
+    apply (unfold empty_iff)
+    apply (rule iffI)
+     apply (drule image_const)
+     apply (drule iffD1[OF all_cong1, rotated])
+      apply (rule sym)
+      apply (rule arg_cong2[OF refl, of _ _ "(\<in>)"])
+      apply (rule FTerm_pre.set_map)
+           apply (rule supp_id_bound bij_id)+
+     apply (subst (asm) eta_natural')
+         apply (rule supp_id_bound bij_id)+
+     apply (unfold id_def)
+     apply (drule forall_in_eq_UNIV)
+     apply (drule trans[symmetric])
+      apply (rule conjunct1[OF card_order_on_Card_order, OF FTerm_pre.bd_card_order])
+     apply (drule card_of_ordIso_subst)
+     apply (drule ordIso_symmetric)
+     apply (drule ordIso_transitive)
+      apply (rule ordIso_symmetric)
+      apply (rule iffD1[OF Card_order_iff_ordIso_card_of])
+      apply (rule conjunct2[OF card_order_on_Card_order, OF FTerm_pre.bd_card_order])
+     apply (erule ordIso_ordLess_False)
+     apply (rule FTerm_pre.set_bd)
+    apply (erule FalseE)
+    done
+  subgoal
+    apply (rule set_eqI)
+    apply (unfold empty_iff)
+    apply (rule iffI)
+     apply (drule image_const)
+     apply (drule iffD1[OF all_cong1, rotated])
+      apply (rule sym)
+      apply (rule arg_cong2[OF refl, of _ _ "(\<in>)"])
+      apply (rule FTerm_pre.set_map)
+           apply (rule supp_id_bound bij_id)+
+     apply (subst (asm) eta_natural')
+         apply (rule supp_id_bound bij_id)+
+     apply (unfold id_def)
+     apply (drule forall_in_eq_UNIV)
+     apply (drule trans[symmetric])
+      apply (rule conjunct1[OF card_order_on_Card_order, OF FTerm_pre.bd_card_order])
+     apply (drule card_of_ordIso_subst)
+     apply (drule ordIso_symmetric)
+     apply (drule ordIso_transitive)
+      apply (rule ordIso_symmetric)
+      apply (rule iffD1[OF Card_order_iff_ordIso_card_of])
+      apply (rule conjunct2[OF card_order_on_Card_order, OF FTerm_pre.bd_card_order])
+     apply (erule ordIso_ordLess_False)
+     apply (rule FTerm_pre.set_bd)
+    apply (erule FalseE)
+    done
+  done
+
+lemma tvsubst_VVr:
+  assumes    
+    "|SSupp_FTerm f1| <o cmin |UNIV::'tv set| |UNIV::'v set|"
+    "|SSupp_FType f2| <o cmin |UNIV::'tv set| |UNIV::'v set|"
+  shows "tvsubst_FTerm f1 f2 (VVr a :: ('tv::var, 'v::var) FTerm) = f1 a"
+  apply (unfold tvsubst_FTerm_def VVr_def comp_def)
+  apply (rule trans)
+   apply (rule FTerm.rec_Uctor)
+      apply (unfold valid_P_def prod.case)
+      apply (rule conjI assms)+
+     apply (unfold eta_set_empties noclash_FTerm_def Uctor_def Un_empty prod.case)
+     apply (rule Int_empty_left conjI)+
+  apply (subst FTerm_pre.map_comp, (rule supp_id_bound bij_id)+)+
+  apply (unfold id_o o_id comp_def[of fst] fst_conv id_def[symmetric] FTerm_pre.map_id)
+  apply (rule trans)
+   apply (rule if_P)
+   apply (unfold isVVr_def VVr_def comp_def )
+   apply (rule exI)
+   apply (rule refl)
+  apply (unfold meta_eq_to_obj_eq[OF VVr_def, THEN fun_cong, unfolded comp_def, symmetric] asVVr_VVr)
+  apply (rule refl)
+  done
+
+lemma tvsubst_FTerm_no_is_VVr:
+  fixes x::"('tv::var, 'v::var) U1_pre"
+  assumes f_prems: "|SSupp_FTerm f1| <o cmin |UNIV::'tv set| |UNIV::'v set|" "|SSupp_FType f2| <o cmin |UNIV::'tv set| |UNIV::'v set|"
+    and empty_prems: "set3_FTerm_pre x \<inter> (IImsupp_FTerm1 f1 \<union> IImsupp_FType f2) = {}" "set4_FTerm_pre x \<inter> IImsupp_FTerm2 f1 = {}"
+    and noclash: "noclash_FTerm x"
+    and VVr_prems: "\<not>isVVr (FTerm_ctor x)"
+  shows
+    "tvsubst_FTerm f1 f2 (FTerm_ctor x) = FTerm_ctor (Sb_FTerm_pre id f2 (map_FTerm_pre id id id id (tvsubst_FTerm f1 f2) (tvsubst_FTerm f1 f2) x))"
+  apply (unfold tvsubst_FTerm_def)
+  apply (subgoal_tac "valid_P (f1, f2)")
+   prefer 2
+   apply (unfold valid_P_def prod.case)[1]
+   apply (rule conjI f_prems)+
+  apply (rule trans)
+   apply (rule FTerm.rec_Uctor)
+      apply assumption
+     apply (unfold PFVars_1_def PFVars_2_def prod.case)
+     apply (rule empty_prems noclash)+
+  apply (unfold Uctor_def prod.case)
+  apply (subst FTerm_pre.map_comp, (rule supp_id_bound bij_id)+)+
+  apply (unfold id_o o_id comp_def[of fst] fst_conv id_def[symmetric] FTerm_pre.map_id)
+  apply (subst if_not_P, rule VVr_prems)+
+  apply (unfold comp_def snd_conv if_P)
+  apply (rule refl)
+  done
+
+(* Sugar theorems for substitution *)
+definition Var :: "'v \<Rightarrow> ('tv::var, 'v::var) FTerm" where
+  "Var a \<equiv> FTerm_ctor (Abs_FTerm_pre (Inl a))"
+definition App :: "('tv, 'v) FTerm \<Rightarrow> ('tv, 'v) FTerm \<Rightarrow> ('tv::var, 'v::var) FTerm" where
+  "App t1 t2 \<equiv> FTerm_ctor (Abs_FTerm_pre (Inr (Inl (t1, t2))))"
+definition TyApp :: "('tv, 'v) FTerm \<Rightarrow> 'tv FType \<Rightarrow> ('tv::var, 'v::var) FTerm" where
+  "TyApp t T \<equiv> FTerm_ctor (Abs_FTerm_pre (Inr (Inr (Inl (t, T)))))"
+definition Lam :: "'v \<Rightarrow> 'tv FType \<Rightarrow> ('tv, 'v) FTerm \<Rightarrow> ('tv::var, 'v::var) FTerm" where
+  "Lam x T t \<equiv> FTerm_ctor (Abs_FTerm_pre (Inr (Inr (Inr (Inl (x, T, t))))))"
+definition TyLam :: "'tv \<Rightarrow> ('tv, 'v) FTerm \<Rightarrow> ('tv::var, 'v::var) FTerm" where
+  "TyLam a t \<equiv> FTerm_ctor (Abs_FTerm_pre (Inr (Inr (Inr (Inr (a, t))))))"
+
+lemma FTerm_subst:
+  fixes f1::"'v \<Rightarrow> ('tv::var, 'v::var) FTerm" and f2::"'tv \<Rightarrow> 'tv FType"
+  assumes "|SSupp_FTerm f1| <o cmin |UNIV::'tv set| |UNIV::'v set|" "|SSupp_FType f2| <o cmin |UNIV::'tv set| |UNIV::'v set|"
+  shows
+    "tvsubst_FTerm f1 f2 (Var x) = f1 x"
+    "tvsubst_FTerm f1 f2 (App t1 t2) = App (tvsubst_FTerm f1 f2 t1) (tvsubst_FTerm f1 f2 t2)"
+    "tvsubst_FTerm f1 f2 (TyApp t T) = TyApp (tvsubst_FTerm f1 f2 t) (tvsubst_FType f2 T)"
+    "x \<notin> IImsupp_FTerm2 f1 \<Longrightarrow> tvsubst_FTerm f1 f2 (Lam x T t) = Lam x (tvsubst_FType f2 T) (tvsubst_FTerm f1 f2 t)"
+    "a \<notin> IImsupp_FTerm1 f1 \<union> IImsupp_FType f2 \<Longrightarrow> tvsubst_FTerm f1 f2 (TyLam a t) = TyLam a (tvsubst_FTerm f1 f2 t)"
+      apply (unfold Var_def App_def TyApp_def Lam_def TyLam_def)
+      apply (unfold meta_eq_to_obj_eq[OF VVr_def, THEN fun_cong, unfolded comp_def, symmetric])
+      apply (rule tvsubst_VVr)
+       apply (rule assms)+
+
+     apply (rule trans)
+      apply (rule tvsubst_FTerm_no_is_VVr)
+           apply (rule assms)+
+         apply (unfold set3_FTerm_pre_def sum.set_map prod.set_map UN_empty2 Un_empty_left Un_empty_right UN_singleton comp_def
+      Abs_FTerm_pre_inverse[OF UNIV_I] sum_set_simps UN_single UN_empty set4_FTerm_pre_def noclash_FTerm_def
+      )
+         apply (rule Int_empty_left conjI)+
+      apply (unfold isVVr_def VVr_def comp_def FTerm.TT_inject0)[1]
+      apply (rule notI)
+      apply (erule exE conjE)+
+      apply (unfold map_FTerm_pre_def comp_def Abs_FTerm_pre_inverse[OF UNIV_I] map_sum.simps prod.map_id
+      Abs_FTerm_pre_inject[OF UNIV_I UNIV_I]
+      )[1]
+      apply (rotate_tac -1)
+      apply (erule contrapos_pp)
+      apply (rule sum.distinct)
+     apply (unfold map_FTerm_pre_def comp_def Abs_FTerm_pre_inverse[OF UNIV_I] map_sum.simps prod.map_id
+      Abs_FTerm_pre_inject[OF UNIV_I UNIV_I] Sb_FTerm_pre_def id_def map_prod_simp
+      )[1]
+     apply (rule refl)
+
+    apply (rule trans)
+     apply (rule tvsubst_FTerm_no_is_VVr)
+          apply (rule assms)+
+        apply (unfold set3_FTerm_pre_def sum.set_map prod.set_map UN_empty2 Un_empty_left Un_empty_right UN_singleton comp_def
+      Abs_FTerm_pre_inverse[OF UNIV_I] sum_set_simps UN_single UN_empty set4_FTerm_pre_def noclash_FTerm_def
+      )
+        apply (rule Int_empty_left conjI)+
+     apply (unfold isVVr_def VVr_def comp_def FTerm.TT_inject0)[1]
+     apply (rule notI)
+     apply (erule exE conjE)+
+     apply (unfold map_FTerm_pre_def comp_def Abs_FTerm_pre_inverse[OF UNIV_I] map_sum.simps prod.map_id
+      Abs_FTerm_pre_inject[OF UNIV_I UNIV_I]
+      )[1]
+     apply (rotate_tac -1)
+     apply (erule contrapos_pp)
+     apply (rule sum.distinct)
+    apply (unfold map_FTerm_pre_def comp_def Abs_FTerm_pre_inverse[OF UNIV_I] map_sum.simps prod.map_id
+      Abs_FTerm_pre_inject[OF UNIV_I UNIV_I] Sb_FTerm_pre_def id_def map_prod_simp bmv_defs
+      )[1]
+    apply (unfold id_def[symmetric] FType.map_id)
+    apply (rule refl)
+
+   apply (rule trans)
+    apply (rule tvsubst_FTerm_no_is_VVr)
+         apply (rule assms)+
+       apply (unfold set2_FTerm_pre_def set6_FTerm_pre_def set3_FTerm_pre_def sum.set_map prod.set_map UN_empty2 Un_empty_left Un_empty_right UN_singleton comp_def
+      Abs_FTerm_pre_inverse[OF UNIV_I] sum_set_simps UN_single UN_empty set4_FTerm_pre_def noclash_FTerm_def prod_set_simps
+      )
+       apply (rule Int_empty_left Int_empty_right conjI iffD2[OF disjoint_single] | assumption)+
+    apply (unfold isVVr_def VVr_def comp_def FTerm.TT_inject0)[1]
+    apply (rule notI)
+    apply (erule exE conjE)+
+    apply (unfold map_FTerm_pre_def comp_def Abs_FTerm_pre_inverse[OF UNIV_I] map_sum.simps prod.map_id
+      Abs_FTerm_pre_inject[OF UNIV_I UNIV_I]
+      )[1]
+    apply (rotate_tac -1)
+    apply (erule contrapos_pp)
+    apply (rule sum.distinct)
+   apply (unfold map_FTerm_pre_def comp_def Abs_FTerm_pre_inverse[OF UNIV_I] map_sum.simps prod.map_id
+      Abs_FTerm_pre_inject[OF UNIV_I UNIV_I] Sb_FTerm_pre_def id_def map_prod_simp bmv_defs
+      )[1]
+   apply (unfold id_def[symmetric] FType.map_id)
+   apply (rule refl)
+
+  apply (rule trans)
+   apply (rule tvsubst_FTerm_no_is_VVr)
+        apply (rule assms)+
+      apply (unfold set2_FTerm_pre_def set6_FTerm_pre_def set3_FTerm_pre_def sum.set_map prod.set_map UN_empty2 Un_empty_left Un_empty_right UN_singleton comp_def
+      Abs_FTerm_pre_inverse[OF UNIV_I] sum_set_simps UN_single UN_empty set4_FTerm_pre_def noclash_FTerm_def prod_set_simps
+      set1_FTerm_pre_def
+      )
+      apply (rule Int_empty_left Int_empty_right conjI iffD2[OF disjoint_single] | assumption)+
+   apply (unfold isVVr_def VVr_def comp_def FTerm.TT_inject0)[1]
+   apply (rule notI)
+   apply (erule exE conjE)+
+   apply (unfold map_FTerm_pre_def comp_def Abs_FTerm_pre_inverse[OF UNIV_I] map_sum.simps prod.map_id
+      Abs_FTerm_pre_inject[OF UNIV_I UNIV_I]
+      )[1]
+   apply (rotate_tac -1)
+   apply (erule contrapos_pp)
+   apply (rule sum.distinct)
+  apply (unfold map_FTerm_pre_def comp_def Abs_FTerm_pre_inverse[OF UNIV_I] map_sum.simps prod.map_id
+      Abs_FTerm_pre_inject[OF UNIV_I UNIV_I] Sb_FTerm_pre_def id_def map_prod_simp bmv_defs
+      )[1]
+  apply (rule refl)
+  done
+
 
 end
